Make capability invocation properties more precise
Better distinguish between the different kinds of capability invocation,
and strengthen requirements, e.g. requiring that capabilities invoked
via indirect sentry are loaded from the address of the sentry plus a
specific offset.  Also require that if an invoked data capability is
written to IDC, then an invoked code capability must be written to PCC.

The monotonicity proof goes through, but the proof tooling for concrete
ISAs still needs fixing.

model/isabelle/Capabilities_lemmas.thy
@@ -87,7 +87,7 @@ inductive_set derivable :: "'cap set \<Rightarrow> 'cap set" for C :: "'cap set"
 | SealEntry:
     "\<lbrakk>c' \<in> derivable C; is_tagged_method CC c';
       \<not>is_sealed_method CC c';
-      is_sentry_method CC (seal_method CC c' otype) \<or> is_indirect_sentry_method CC (seal_method CC c' otype)\<rbrakk> \<Longrightarrow>
+      is_sentry_method CC (seal_method CC c' otype) \<or> is_indirect_sentry CC (seal_method CC c' otype)\<rbrakk> \<Longrightarrow>
      seal_method CC c' otype \<in> derivable C"
 
 lemma derivable_mono:
